core/Utils.v
@@ -24,5 +24,12 @@ Definition conjunction {A : Type} (f : A -> bool) (l : list A) : bool :=
   fold_left (fun b x => b && f x) l true
 .
 
+Lemma conjunction_couples :
+  forall {A : Type} (f1 f2: A -> bool) (l : list A),
+    conjunction (fun x => f1 x && f2 x) l = conjunction f1 l && conjunction f2 l
+.
+Proof.
+Admitted.
+
 Definition set_of_list {A : Type} (dec : forall x y : A, {x = y} + {x <> y}) (l : list A) : set A :=
   fold_right (fun x s => if set_mem dec x s then s else x :: s) nil l.
